# 回归算法

$$
y
= \left[ \begin{array}
{c} y_1 \\ \vdots \\ y_n
\end{array}\right]
=\left[y_{1}, \cdots, y_{n}\right]^{T} 
$$

$$
\Phi = \left[\phi(x_1), \cdots, \phi(x_n)\right]
$$

$$
X=\left[x_1, \cdots,x_n\right]
$$







## 1、least-squares (LS)

objective function $\left\|y-\Phi^{T} \theta\right\|^{2}$
$$
\begin{align}
\underset{\theta}{argmin} \left\|y-\Phi^{T} \theta\right\|^{2}
&= \underset{\theta}{argmin} (y-\Phi^T\theta)^T(y-\Phi^T\theta) \\
&= \underset{\theta}{argmin} (y^T-\theta^T\Phi)(y-\Phi^T\theta) \\
&= \underset{\theta}{argmin} [y^Ty-y^T\Phi^T\theta-\theta^T\Phi y+\theta^T\Phi\Phi^T\theta] \\
(都是实数，所以A^T=A)&= \underset{\theta}{argmin} [y^Ty-2y^T\Phi^T\theta+\theta^T\Phi\Phi^T\theta]
\end{align}
$$
derivatives
$$
\frac{\partial}{\partial\theta}[y^Ty-2y^T\Phi^T\theta+\theta^T\Phi\Phi^T\theta]
= -2\Phi y +2\Phi \Phi^T
$$
because $\frac{\partial x^T a}{\partial{x}}=\frac{\partial a^T x}{\partial{x}} = a $ 

